Example traces

TraceSemantics.v
@@ -41,11 +41,16 @@ Fixpoint Stmt_sub (s:Stmt) (u y:LVar) : Stmt :=
   | SGAsgn x e => SGAsgn x (Aapply Gid_sub t e)
   | SLAsgn x e => SLAsgn (if u =? x then y else x) (Aapply Gid_sub t e)
   | SProc P e => SProc P (Aapply Gid_sub t e)
-  | SSeq s1 s2 => SSeq (Stmt_sub s1 u y) (Stmt_sub s1 u y)
+  | SSeq s1 s2 => SSeq (Stmt_sub s1 u y) (Stmt_sub s2 u y)
   | SIf b s1 s2 => SIf (Bapply Gid_sub t b) (Stmt_sub s1 u y) (Stmt_sub s1 u y)
   | SWhile b s => SWhile (Bapply Gid_sub t b) (Stmt_sub s u y)
   | SReturn => SReturn
   end.
+
+
+Definition X : GVar := "X".
+Definition Y : LVar := "Y".
+Definition U : LVar := "U".
 
 Open Scope list_scope.
 
@@ -67,7 +72,7 @@ Inductive Sstep : relation SConfig  :=
     (<{ x :=L e ; s }>, t) ->s (s, t ++ [asgnL x e])
 | SProc_step : forall (t:STrace) u y body e s t,
     (* "y fresh", somehow *)
-    (<{ proc(u){body}(e) ; s }>, t) ->s (SSeq (Stmt_sub body u y) s, t ++ [asgnL u e])
+    (<{ proc(u){body}(e) ; s }>, t) ->s (SSeq (Stmt_sub body u y) s, t ++ [asgnL y e])
 | SReturn_step : forall s t,
     (<{ return ; s }>, t) ->s (s, t)
 | SIfTrue_step : forall b s1 s2 s t,
@@ -106,7 +111,7 @@ Definition acc_GVal' (t:CTrace) (x:GVar) : option nat :=
   fold_left (accG x) t None.
 
 Definition acc_LVal' (t:CTrace) (x:LVar) : option nat :=
-  fold_left (accG x) t None.
+  fold_left (accL x) t None.
 
 (* for now, let's just "cheat" in totality *)
 Definition acc_GVal (t:CTrace) : GVal :=
@@ -116,7 +121,7 @@ Definition acc_GVal (t:CTrace) : GVal :=
         end.
 
 Definition acc_LVal (t:CTrace) : LVal :=
-  fun x => match acc_GVal' t x with
+  fun x => match acc_LVal' t x with
         | None => 0
         | Some n => n
         end.
@@ -132,9 +137,9 @@ Definition CConfig : Type := Stmt * CTrace.
 Reserved Notation " c '=>c' c' " (at level 40).
 
 Inductive Cstep : relation CConfig :=
-| CGASgn_step : forall x e s t,
+| CGAsgn_step : forall x e s t,
     (<{ x :=G e ; s }>, t) =>c (s, t ++ [inl (x, Aeval_t t e)])
-| CLASgn_step : forall x e s t,
+| CLAsgn_step : forall x e s t,
     (<{ x :=L e ; s }>, t) =>c (s, t ++ [inr (x, Aeval_t t e)])
 | CProc_step : forall u body e s t y,
     (<{ proc(u){body}(e) ; s }>, t) =>c (SSeq (Stmt_sub body u y) s, t ++ [inr (y, Aeval_t t e)])
@@ -156,3 +161,76 @@ Inductive Cstep : relation CConfig :=
 
 Definition multi_Cstep := clos_refl_trans_n1 _ Cstep.
 Notation " c '=>*' c' " := (multi_Cstep c c') (at level 40).
+
+Example test_program : Stmt :=
+  <{proc(U){ U :=L U + 1;
+              X :=G U + 2;
+              return}
+       (X + 1);
+     X :=G 0}>.
+
+Lemma app_rewrite3 : forall A (a b c : A),
+    [a ; b ; c] = [a ; b] ++ [c].
+Proof. intros. reflexivity. Qed.
+
+Lemma app_rewrite2 : forall A (a b : A),
+    [a ; b] = [a] ++ [b].
+Proof. intros. reflexivity. Qed.
+
+Lemma app_rewrite1 : forall A (a : A),
+    [a] = [] ++ [a].
+Proof. intros. reflexivity. Qed.
+
+Lemma test_body_subst :
+    <{ Y :=L Y + 1;
+       X :=G Y + 2;
+       return}>
+    = Stmt_sub <{ U :=L U + 1;
+                  X :=G U + 2;
+                  return}>
+        U Y.
+Proof. simpl. rewrite L_single_update. reflexivity. Qed.
+
+(* not sure how to elegantly incorporate this assumption without semantics *)
+Lemma seq_assoc : forall s1 s2 s3,
+    <{(s1; s2); s3}> = <{s1 ; (s2 ; s3)}>. Admitted.
+
+Example Stest_trace : (test_program, [])
+                        ->* (<{X :=G 0}>,
+                                [inr (Y, <{X + 1}>);
+                                  inr (Y, <{Y + 1}>);
+                                  inl (inr (X, <{Y + 2}>))]).
+Proof.
+  eapply Relation_Operators.rtn1_trans. apply SReturn_step.
+  eapply Relation_Operators.rtn1_trans. rewrite app_rewrite3. apply SGAsgn_step.
+  eapply Relation_Operators.rtn1_trans. rewrite app_rewrite2. apply SLAsgn_step.
+  eapply Relation_Operators.rtn1_trans. rewrite app_rewrite1.
+  assert (<{ Y :=L Y + 1; X :=G Y + 2; return; X :=G 0 }> = <{ (Y :=L Y + 1; X :=G Y + 2; return); X :=G 0 }>). {
+    repeat (rewrite seq_assoc). reflexivity. }
+  rewrite H. rewrite test_body_subst. apply SProc_step.
+  exact [].
+  apply rtn1_refl.
+Qed.
+
+Example Ctest_trace : (test_program, [])
+                        =>* (<{X :=G 0}>,
+                                [inr (Y, 1) ;
+                                  inr (Y, 2);
+                                 inl (X, 4)]).
+Proof.
+  eapply Relation_Operators.rtn1_trans. apply CReturn_step.
+  assert (step1 : (test_program, []) =>c (<{Y :=L Y + 1; X :=G Y + 2; return ; X :=G 0}>, [inr (Y, 1)])).
+  {assert (<{ Y :=L Y + 1; X :=G Y + 2; return; X :=G 0 }> = <{ (Y :=L Y + 1; X :=G Y + 2; return); X :=G 0 }>). {
+    repeat (rewrite seq_assoc). reflexivity. }
+    rewrite app_rewrite1. rewrite H. rewrite test_body_subst. apply CProc_step. }
+  assert (step2 : (<{Y :=L Y + 1; X :=G Y + 2; return ; X :=G 0}>, [inr (Y, 1)])
+          =>c (<{ X :=G Y + 2; return; X :=G 0}>, [inr (Y,1) ; inr (Y, 2)])).
+  { rewrite app_rewrite2. apply CLAsgn_step. }
+  assert (step3 : (<{ X :=G Y + 2; return; X :=G 0}>, [inr (Y,1) ; inr (Y, 2)])
+          =>c (<{return; X :=G 0}>, [inr (Y,1) ; inr (Y, 2) ; inl (X, 4)])).
+  { rewrite app_rewrite3. apply CGAsgn_step. }
+  eapply Relation_Operators.rtn1_trans. apply step3.
+  eapply Relation_Operators.rtn1_trans. apply step2.
+  eapply Relation_Operators.rtn1_trans. apply step1.
+  apply rtn1_refl.
+Qed.
